# Math

$$
\begin{aligned}
& P_1 + t_1 V_1 = P_2 + t_2 V_2 \\
& P_{1x} + t_1 V_{1x} = P_{2x} + t_2 V_{2x} \\
& P_{1y} + t_1 V_{1y} = P_{2y} + t_2 V_{2y} \\
& t_1 V_{1x} - t_2 V_{2x} = P_{2x} - P_{1x} \\
& t_1 V_{1y} - t_2 V_{2y} = P_{2y} - P_{1y} \\
& \begin{pmatrix} V_{1x} & -V_{2x} \\ V_{1y} & -V_{2y} \end{pmatrix} \cdot
\begin{pmatrix} t_1 \\ t_2 \end{pmatrix} =
\begin{pmatrix} P_{2x} - P_{1x} \\ P_{2y} - P_{1y} \end{pmatrix} \\
& \bold V \cdot \bold T = \bold P \\
& \bold V^{-1} \cdot \bold V \cdot \bold T = \bold V^{-1} \cdot \bold P \\
& \bold T = \bold V^{-1} \cdot \bold P
\end{aligned}
$$
